DataflowRewriter/Rewrites/CombineMux.lean
@@ -17,8 +17,8 @@ def matcher (T T' : String) (g : ExprHigh String) : RewriteResult (List String) 
       unless typ = "fork Bool 2" do return none
       let (.some mux_nn) := followOutput g inst "out0" | return none
       let (.some mux_nn') := followOutput g inst "out1" | return none
-      unless mux_nn.typ = "mux " ++ T && mux_nn.inputPort = "inp2" do return none
-      unless mux_nn'.typ = "mux " ++ T' && mux_nn'.inputPort = "inp2" do return none
+      unless mux_nn.typ = "mux " ++ T && mux_nn.inputPort = "inp0" do return none
+      unless mux_nn'.typ = "mux " ++ T' && mux_nn'.inputPort = "inp0" do return none
       return some [mux_nn.inst, mux_nn'.inst, inst]
     ) none | throw .done
   return list
@@ -36,22 +36,24 @@ def lhs (T T' : Type) (Tₛ T'ₛ : String) : ExprHigh String × IdentMap String
     mux2 [typeImp = $(⟨_, mux T'⟩), type = $("mux " ++ T'ₛ)];
     condFork [typeImp = $(⟨_, fork Bool 2⟩), type = "fork Bool 2"];
 
-    mux1 -> b1_o [out="out0"];
-    mux2 -> b2_o [out="out0"];
+    mux1 -> b1_o [from="out0"];
+    mux2 -> b2_o [from="out0"];
 
-    cond_i -> condFork [inp="inp0"];
-    b1_t_i -> mux1 [inp="inp0"];
-    b1_f_i -> mux1 [inp="inp1"];
-    b2_t_i -> mux2 [inp="inp0"];
-    b2_f_i -> mux2 [inp="inp1"];
+    cond_i -> condFork [to="inp0"];
+    b1_t_i -> mux1 [to="inp1"];
+    b1_f_i -> mux1 [to="inp2"];
+    b2_t_i -> mux2 [to="inp1"];
+    b2_f_i -> mux2 [to="inp2"];
 
-    condFork -> mux1 [out="out0", inp="inp2"];
-    condFork -> mux2 [out="out1", inp="inp2"];
+    condFork -> mux1 [from="out0", to="inp0"];
+    condFork -> mux2 [from="out1", to="inp0"];
   ]
 
 -- #reduce lhs Unit Unit "H" "Y"
 
 def lhs_extract T₁ T₂ := (lhs Unit Unit T₁ T₂).fst.extract ["mux1", "mux2", "condFork"] |>.get rfl
+
+#eval IO.print (lhs_extract "T" "T'").fst
 
 theorem lhs_type_independent a b c d T₁ T₂ : (lhs a b T₁ T₂).fst = (lhs c d T₁ T₂).fst := by rfl
 
@@ -73,22 +75,24 @@ def rhs (T T' : Type) (Tₛ Tₛ' : String) : ExprHigh String × IdentMap String
     mux [typeImp = $(⟨_, mux (T × T')⟩), type = $("mux (" ++ Tₛ ++ " × " ++ Tₛ' ++ ")")];
     split [typeImp = $(⟨_, split T T'⟩), type = $("split " ++ Tₛ ++ " " ++ Tₛ')];
 
-    b1_t_i -> joinT [inp="inp0"];
-    b2_t_i -> joinT [inp="inp1"];
-    b1_f_i -> joinF [inp="inp0"];
-    b2_f_i -> joinF [inp="inp1"];
+    b1_t_i -> joinT [to="inp0"];
+    b2_t_i -> joinT [to="inp1"];
+    b1_f_i -> joinF [to="inp0"];
+    b2_f_i -> joinF [to="inp1"];
 
-    cond_i -> mux [inp="inp2"];
+    cond_i -> mux [to="inp0"];
 
-    joinT -> mux [out="out0", inp="inp0"];
-    joinF -> mux [out="out0", inp="inp1"];
-    mux -> split [out="out0", inp="inp0"];
+    joinT -> mux [from="out0", to="inp1"];
+    joinF -> mux [from="out0", to="inp2"];
+    mux -> split [from="out0", to="inp0"];
 
-    split -> b1_o [out="out0"];
-    split -> b2_o [out="out1"];
+    split -> b1_o [from="out0"];
+    split -> b2_o [from="out1"];
   ]
 
 def rhsLower T₁ T₂ := (rhs Unit Unit T₁ T₂).fst.lower.get rfl
+
+#eval IO.print ((rhs Unit Unit "T" "T'").fst)
 
 theorem rhs_type_independent a b c d T₁ T₂ : (rhs a b T₁ T₂).fst = (rhs c d T₁ T₂).fst := by rfl
 
